fstar/treesync/proofs/MLS.TreeSync.Invariants.ParentHash.Proofs.fst
@@ -1,5 +1,6 @@
 module MLS.TreeSync.Invariants.ParentHash.Proofs
 
+open FStar.List.Tot
 open Comparse
 open MLS.Crypto
 open MLS.NetworkTypes
@@ -199,6 +200,240 @@ let mem_last_update_rhs_eq #bytes #bl #tkt #ld #lp #id #ip d p x =
   let (|xl, xi|) = x in
   mem_unmerged_resolution_eq (List.Tot.filter (leaf_index_inside_tree c) p_unmerged_leaves) x;
   mem_ul_filter (leaf_index_inside_tree c) p_unmerged_leaves xi
+
+(*** last_update set equality imply equality ***)
+
+val unmerged_leaves_sorted_filter_head:
+  p:(nat_lbytes 4 -> bool) -> l:list(nat_lbytes 4) ->
+  Lemma
+  (requires unmerged_leaves_sorted l)
+  (ensures (
+    match l, List.Tot.filter p l with
+    | h1::_, h2::_ -> h1 <= h2
+    | _, _ -> True
+  ))
+let rec unmerged_leaves_sorted_filter_head p l =
+  match l with
+  | [] -> ()
+  | h::t -> unmerged_leaves_sorted_filter_head p t
+
+val unmerged_leaves_sorted_filter:
+  p:(nat_lbytes 4 -> bool) -> l:list(nat_lbytes 4) ->
+  Lemma
+  (requires unmerged_leaves_sorted l)
+  (ensures unmerged_leaves_sorted (List.Tot.filter p l))
+let rec unmerged_leaves_sorted_filter p l =
+  match l with
+  | [] -> ()
+  | h::t ->
+    unmerged_leaves_sorted_filter p t;
+    if p h then unmerged_leaves_sorted_filter_head p t
+    else ()
+
+val node_indices_are_leaf_indices:
+  list node_index ->
+  prop
+let node_indices_are_leaf_indices ll =
+  forall l i. List.Tot.memP (|l, i|) ll ==> l == 0
+
+val node_index_to_tree_index: node_index -> nat
+let node_index_to_tree_index (|_, i|) = i
+
+val node_indices_are_sorted:
+  list node_index ->
+  bool
+let rec node_indices_are_sorted l =
+  match l with
+  | [] -> true
+  | [_] -> true
+  | h1::h2::t -> (
+    node_index_to_tree_index h1 < node_index_to_tree_index h2 &&
+    node_indices_are_sorted (h2::t)
+  )
+
+#push-options "--fuel 2 --ifuel 1"
+val unmerged_resolution_unmerged_leaves_sorted:
+  l:list (nat_lbytes 4) ->
+  Lemma
+  (requires unmerged_leaves_sorted l)
+  (ensures
+    node_indices_are_leaf_indices (unmerged_resolution l) /\
+    node_indices_are_sorted (unmerged_resolution l)
+  )
+let rec unmerged_resolution_unmerged_leaves_sorted l =
+  match l with
+  | [] -> ()
+  | [_] -> ()
+  | h1::h2::t -> unmerged_resolution_unmerged_leaves_sorted (h2::t)
+#pop-options
+
+#push-options "--fuel 2 --ifuel 1"
+val node_indices_are_sorted_append:
+  l1:list node_index -> l2:list node_index -> cutoff: nat ->
+  Lemma
+  (requires
+    node_indices_are_sorted l1 /\
+    node_indices_are_sorted l2 /\
+    (forall xl xi. List.Tot.memP (|xl, xi|) l1 ==> xi < cutoff) /\
+    (forall xl xi. List.Tot.memP (|xl, xi|) l2 ==> cutoff <= xi)
+  )
+  (ensures node_indices_are_sorted (l1@l2))
+let rec node_indices_are_sorted_append l1 l2 cutoff =
+  match l1 with
+  | [] -> ()
+  | [h] -> (
+    match l2 with
+    | [] -> ()
+    | h2::t2 -> ()
+  )
+  | h1::h2::t ->
+    node_indices_are_sorted_append (h2::t) l2 cutoff
+#pop-options
+
+val node_indices_are_sorted_filter_head:
+  p:(node_index -> bool) -> l:list node_index ->
+  Lemma
+  (requires node_indices_are_sorted l)
+  (ensures (
+    match l, List.Tot.filter p l with
+    | h1::_, h2::_ -> node_index_to_tree_index h1 <= node_index_to_tree_index h2
+    | _, _ -> True
+  ))
+let rec node_indices_are_sorted_filter_head p l =
+  match l with
+  | [] -> ()
+  | h::t -> node_indices_are_sorted_filter_head p t
+
+val node_indices_are_sorted_filter:
+  p:(node_index -> bool) -> l:list(node_index) ->
+  Lemma
+  (requires node_indices_are_sorted l)
+  (ensures node_indices_are_sorted (List.Tot.filter p l))
+let rec node_indices_are_sorted_filter p l =
+  match l with
+  | [] -> ()
+  | h::t ->
+    node_indices_are_sorted_filter p t;
+    if p h then node_indices_are_sorted_filter_head p t
+    else ()
+
+#push-options "--fuel 2 --ifuel 1"
+val filtered_resolution_are_leaves_imply_are_sorted:
+  #bytes:Type0 -> {|bytes_like bytes|} -> #tkt:treekem_types bytes ->
+  #l:nat -> #i:tree_index l ->
+  p:(node_index -> bool) -> t:treesync bytes tkt l i ->
+  Lemma
+  (requires
+    node_indices_are_leaf_indices (List.Tot.filter p (resolution t)) /\
+    unmerged_leaves_ok t
+  )
+  (ensures node_indices_are_sorted (List.Tot.filter p (resolution t)))
+let rec filtered_resolution_are_leaves_imply_are_sorted #bytes #bl #tkt #l #i p t =
+  match t with
+  | TLeaf _ -> ()
+  | TNode None left right -> (
+    filter_append p (resolution left) (resolution right);
+    FStar.Classical.forall_intro (List.Tot.append_mem (List.Tot.filter p (resolution left)) (List.Tot.filter p (resolution right)));
+    filtered_resolution_are_leaves_imply_are_sorted p left;
+    filtered_resolution_are_leaves_imply_are_sorted p right;
+    FStar.Classical.forall_intro (mem_filter p (resolution left));
+    FStar.Classical.forall_intro (mem_filter p (resolution right));
+    FStar.Classical.forall_intro (FStar.Classical.move_requires (resolution_inside_tree left));
+    FStar.Classical.forall_intro (FStar.Classical.move_requires (resolution_inside_tree right));
+    node_indices_are_sorted_append (List.Tot.filter p (resolution left)) (List.Tot.filter p (resolution right)) (i + pow2 (l-1))
+  )
+  | TNode (Some content) _ _ -> (
+    unmerged_resolution_unmerged_leaves_sorted content.unmerged_leaves;
+    node_indices_are_sorted_filter p (unmerged_resolution content.unmerged_leaves)
+  )
+#pop-options
+
+val last_update_lhs_sorted:
+  #bytes:Type0 -> {|bytes_like bytes|} -> #tkt:treekem_types bytes ->
+  #ld:nat -> #lp:nat{ld < lp} -> #id:tree_index ld -> #ip:tree_index lp{leaf_index_inside lp ip id} ->
+  d:treesync bytes tkt ld id -> p:treesync bytes tkt lp ip{node_not_blank p} ->
+  Lemma
+  (requires
+    node_indices_are_leaf_indices (last_update_lhs d p) /\
+    unmerged_leaves_ok p
+  )
+  (ensures
+    node_indices_are_sorted (last_update_lhs d p)
+  )
+let last_update_lhs_sorted #bytes #bl #tkt #ld #lp #id #ip d p =
+  let (c, _) = get_child_sibling p id in
+  filtered_resolution_are_leaves_imply_are_sorted (op_disEquality (|ld, id|)) c
+
+val last_update_rhs_sorted:
+  #bytes:Type0 -> {|bytes_like bytes|} -> #tkt:treekem_types bytes ->
+  #ld:nat -> #lp:nat{ld < lp} -> #id:tree_index ld -> #ip:tree_index lp{leaf_index_inside lp ip id} ->
+  d:treesync bytes tkt ld id -> p:treesync bytes tkt lp ip{node_not_blank p} ->
+  Lemma
+  (requires unmerged_leaves_ok p)
+  (ensures
+    node_indices_are_leaf_indices (last_update_rhs d p) /\
+    node_indices_are_sorted (last_update_rhs d p)
+  )
+let last_update_rhs_sorted #bytes #bl #tkt #ld #lp #id #ip d p =
+  let (c, _) = get_child_sibling p id in
+  let p_unmerged_leaves = (Some?.v (TNode?.data p)).unmerged_leaves in
+  unmerged_leaves_sorted_filter (leaf_index_inside_tree c) p_unmerged_leaves;
+  unmerged_resolution_unmerged_leaves_sorted (List.Tot.filter (leaf_index_inside_tree c) p_unmerged_leaves)
+
+val node_indices_are_sorted_less_than_head:
+  x:node_index -> l:list node_index ->
+  Lemma
+  (requires
+    node_indices_are_sorted l /\ (
+      match l with
+      | [] -> True
+      | h::t -> node_index_to_tree_index x < node_index_to_tree_index h
+    )
+  )
+  (ensures forall y. List.Tot.memP y l ==> node_index_to_tree_index x < node_index_to_tree_index y)
+let rec node_indices_are_sorted_less_than_head x l =
+  match l with
+  | [] -> ()
+  | h::t -> node_indices_are_sorted_less_than_head x t
+
+val node_indices_are_leaf_indices_and_sorted_set_eqP_imply_eq:
+  l1:list node_index -> l2:list node_index ->
+  Lemma
+  (requires
+    node_indices_are_leaf_indices l1 /\
+    node_indices_are_leaf_indices l2 /\
+    node_indices_are_sorted l1 /\
+    node_indices_are_sorted l2 /\
+    set_eqP l1 l2
+  )
+  (ensures l1 == l2)
+let rec node_indices_are_leaf_indices_and_sorted_set_eqP_imply_eq l1 l2 =
+  match l1, l2 with
+  | [], [] -> ()
+  | [], h2::t2 -> assert(False)
+  | h1::t1, [] -> assert(False)
+  | h1::t1, h2::t2 -> (
+    node_indices_are_sorted_less_than_head h1 t1;
+    node_indices_are_sorted_less_than_head h2 t2;
+    node_indices_are_leaf_indices_and_sorted_set_eqP_imply_eq t1 t2
+  )
+
+#push-options "--fuel 0 --ifuel 0"
+val last_update_set_eqP_imply_eq:
+  #bytes:Type0 -> {|bytes_like bytes|} -> #tkt:treekem_types bytes ->
+  #ld:nat -> #lp:nat{ld < lp} -> #id:tree_index ld -> #ip:tree_index lp{leaf_index_inside lp ip id} ->
+  d:treesync bytes tkt ld id -> p:treesync bytes tkt lp ip{node_not_blank p} ->
+  Lemma
+  (requires
+    unmerged_leaves_ok p /\
+    set_eqP (last_update_lhs d p) (last_update_rhs d p)
+  )
+  (ensures (last_update_lhs d p) == (last_update_rhs d p))
+let last_update_set_eqP_imply_eq #bytes #bl #tkt #ld #lp #id #ip d p =
+  last_update_rhs_sorted d p;
+  last_update_lhs_sorted d p;
+  node_indices_are_leaf_indices_and_sorted_set_eqP_imply_eq (last_update_lhs d p) (last_update_rhs d p)
+#pop-options
 
 (*** prop invariant definition ***)
 
